\section{Converting Spectra Between Coordinate Systems}
\label{sec:Apx_ConvertingSpectra}

The Jacobian of the coordinate change to Bjorken coordinates is
\begin{equation}
    \big\vert\frac{\partial(m_T,p_T,\eta_p,\varphi_o)}{\partial(p^x,p^y,p^z,p^t)}\big\vert=\frac{1}{m_T p_T}
\end{equation}
Let $f(p^\mu)$ be some distribution function and $F$ its momentum space integral evaluated on the momentum shell and future directed momenta.

\begin{subequations}
    \begin{align}
        F&=\int\frac{\dt^4p_{\text{cart}}}{(2\pi)^4}\delta(p^2+m^2)\Theta(p^t)f(p^\mu)\\
        & =\int\frac{\dt p^t}{2\pi}\int\frac{\dt^3p_{\text{cart}}}{(2\pi)^3}\frac{1}{2\omega_{\vec{p}}}\big(\delta(p^t-\omega_{\vec{p}})+\delta(p^t+\omega_{\vec{p}})\big)\Theta(p^t)f(p^\mu) \\
                                                                                      & =\frac{1}{2\pi}\int\frac{\dt^3p_{\text{cart}}}{(2\pi)^3}\frac{1}{2\omega_{\vec{p}}}f(p^\mu)\big\vert_{p^t=\omega_{\vec{p}}}\\
    \intertext{On the other hand}
        F&=\int\frac{\dt^4p_{\text{cart}}}{(2\pi)^4}\delta(p^2+m^2)\Theta(p^t)f(p^\mu)\\
        & =\frac{1}{(2\pi)^4}\int_0^\infty \dt p_T\int_0^\infty \dt m_T\int_{-\infty}^\infty \dt\eta_p\int_0^{2\pi}\dt\varphi_pm_T p_T\times\nonumber \\
                                                                                      & \phantom{=}\qquad\times\delta((p_T)^2-(m_T)^2+m^2)f(p^\mu)\,.                                                                                              \\
        \intertext{Assume $f(p^\mu)=f(p_T,m_T,\eta_p)$ and perform the $\varphi_p$-integraion as well as $m_T$-integration, where $\omega_T^2=m^2+p_T^2$ to find}
                                                                                      \dots& =\frac{1}{(2\pi)^3}\int_0^\infty\dt p_T\int_{-\infty}^\infty\dt\eta_p\frac{p_T}{2}f(p^\mu)\big\vert_{m_T=\omega_T}\,,
    \end{align}
    leading to the final result
    \begin{equation}
        \frac{1}{2\pi}\int\frac{\dt^3p_{\text{cart}}}{(2\pi)^3}\frac{1}{2\omega_{\vec{p}}}f(p^\mu)\big\vert_{p^t=\omega_{\vec{p}}}=\frac{1}{(2\pi)^3}\int_0^\infty\dt p_T\int_{-\infty}^\infty\dt\eta_p\frac{p_T}{2}f(p^\mu)\big\vert_{m_T=\omega_T}
    \end{equation}
\end{subequations}
Since the restrictions $p^t=\omega_{\vec{p}}$ and $m_T=\omega_T$ are equivalent (considering the parametrization that already satisfies $p^t=p_T\cosh\eta_p\geq 0$) we find
\begin{equation}
    \omega_{\vec{p}}\frac{\dt F}{\dt p^x\dt p^y\dt p^z}=\frac{1}{2\pi p_T}\frac{\dt F}{\dt p_T\dt\eta_p}
\end{equation}
The result applies to the case
\begin{equation}
    f(p^\mu)\big\vert_{p^t=\omega_{\vec{p}}}=2\omega_{\vec{p}}\cdot 2\pi\cdot n(\vec{p})
\end{equation}
and $F=N$. This holds for the symmetric range $\eta\in(-\infty,\infty)$. If $f$ is symmetric under ${\eta\to -\eta}$, restricting to $\eta\in[0,\infty)$ we find
\begin{equation}
    2\omega_{\vec{p}}\frac{\dt F}{\dt p^x\dt p^y\dt p^z}=\frac{1}{2\pi p_T}\frac{\dt F}{\dt p_T\dt\eta_p}\,.
\end{equation}