\chapter{Calculation of Condensed Field}

\section{Finding the Condensate of the Freeze-Out Surface}

The freeze-out surface is invariant under rotations (= independent of polar angle $\varphi$) around the collision axis and longitudinal boosts (= independent of rapidity $\eta_s$) and hence parametrized by a one-dimensional curve in the $r\text{-}\tau$-plane. The curve itself may be parametrized by some real parameter $\alpha$, following some mapping $s\mapsto (r(\alpha),\tau(\alpha))$. From the hydro simulation we wish to identify the gradient $\partial_\mu\vartheta\sim u_\mu$ of the complex phase of the condensate field with the fluid $4$-velocity $u_\mu$, hence in order to find the phase of the field, an integration of $\partial_\mu\vartheta$ over the hypersurface is needed and an integration constant $\vartheta_0$ can be chosen freely. Choose $\alpha=\arctan(y/x)$ to be the polar angle of the point $(r(\alpha),\tau(\alpha))$ in the $r\text{-}\tau$-plane. Since $r,\tau>0$ $\alpha$ is restricted to the range $[0,\pi]$ and $\vartheta(\alpha)$ on the hypersurface can be calculated via
\begin{equation}
    \vartheta(\alpha)=\vartheta_0+\int_0^\alpha\dt s\frac{\dt\vartheta}{\dt s}=\vartheta_0+\int_0^\alpha\dt s\frac{\partial x^\mu(s)}{\partial s}\partial_\mu\vartheta
\end{equation}
$\partial x^\mu(s)/\partial s$ represents the tangent vector of the freeze-out surface.

The energy density $\epsilon$ and $4$-velocity $u^\mu$ of the fluid is related to the condensate phase and density via
\begin{subequations}
    \begin{gather}
        -(\partial_\mu\vartheta)(\partial^\mu\vartheta)=\chi^2=\frac{-\mu^2+\sqrt{6\epsilon\lambda+2\mu^4}}{3}\\
        \partial^\mu\vartheta=\chi u^\mu\,,\qquad\rho^2=\sqrt{\frac{\chi^2+\mu^2}{\lambda}}
    \end{gather}
\end{subequations}
One may use the relations \eqref{eq:LinearSigmaModel_CouplingsMassesRelation} to rewrite the above equation in terms of the particle masses and the pion decay constant $f_\pi\equiv v$.
\begin{equation}
    \chi^2=\frac{-m_\sigma^2/2+\sqrt{3\epsilon m_\sigma^2/f_\pi+m_\sigma^4/2}}{3}=\frac{-m_\sigma^2+m_\sigma\sqrt{12\epsilon/f_\pi+2m_\sigma^2}}{6}\,,\qquad\rho=\sqrt{f_\pi\frac{2\chi^2+m_\sigma^2}{m_\sigma^2}}
\end{equation}

In Milne coordinates $(x^\mu)=(\tau,r,\varphi,\eta_s)$ the $4$-velocity has components $(u^\mu)=(\gamma,\gamma v,0,0)$, where $v=v(\alpha)$ is a function on the freeze-out surface.

Questions to Andreas regarding numerics:
\begin{itemize}
    \item Why is $\dt\alpha=\alpha_{j+1}-\alpha_{j}\neq\const$?
\end{itemize}

\section{Finding the Spectrum at the Detector Surface}

In general the particle number $N$ and particle number density $n(\mathbf{x})$ in position space and $n(\mathbf{p})$ in momentum space associated to the condensate $\phi(\mathbf{x})$ of a complex scalar field are given by the relations
\begin{subequations}
    \begin{gather}
        n(\mathbf{x})=\phi(\mathbf{x})\phi^*(\mathbf{x})\,,\qquad n(\mathbf{p})=\phi(\mathbf{p})\phi^*(\mathbf{p})\\
        N=\int\dt^3xn(\mathbf{x})=\int\frac{\dt^3p}{(2\pi)^3}n(\mathbf{p})
    \end{gather}
\end{subequations}
with the convention $\phi(\mathbf{x})=\int\dt^3p/(2\pi)^3\phi(\mathbf{p})e^{-\imagu\mathbf{p}\mathbf{x}}$ for the Fourier transform.


% The field configuration found by this translation prescription is then propagated forwards in time by means of the retarded Greens function
% \begin{equation}
%     \overline{\phi}(x)=\langle\phi_a(x)\rangle=\int\dt^dyG_{\text{ret}}(x,y)j(y)
% \end{equation}
% $j(y)$ is defined to be the field configruation on the freezout surface. The retarded Greens function is given by $G_{\text{ret}}(x,y)=\Theta(x^0-y^0)\big(D(x-y)-D(y-x)\big)$ where
% \begin{equation}
%     D(\Delta x)=\int\frac{\dt^3p}{(2\pi)^3}\frac{1}{2\omega_\mathbf{p}}e^{-\imagu(\omega_\mathbf{p}\Delta t-\mathbf{p}\Delta\mathbf{x})}
% \end{equation}
% and $\omega_\mathbf{p}=\sqrt{m^2+\mathbf{p}^2}$.

\includepdf{resources/notes_0430.pdf}

\subsection{Treating the Freeze Out Field as Source Term}

Let's evaluate the Fourier transform of the condensate field. The calculation uses the result from linear response theory
\begin{subequations}
    \begin{equation}
        \overline{\phi}(x)\equiv\langle\phi(x)\rangle=\int\dt^4G_{\text{ret}}(x,y)j(y)
    \end{equation}
    for a source term $j(y)$. The retarded Greens function is given by
    \begin{equation}
        G_{\text{ret}}(x,y)=\Theta(x^0-y^0)\big[D(x-y)-D(y-x)\big]
    \end{equation}
    with the propagator
    \begin{equation}
        D(x-y)=\int\frac{\dt^3q}{(2\pi)^3}\frac{e^{-\imagu[\omega_{\mathbf{q}}(x^0-y^0)-\mathbf{q}(\mathbf{x}-\mathbf{y})]}}{2\omega_{\mathbf{q}}}
    \end{equation}
    and the relations
    \begin{equation}
        \int\dt^3x e^{\imagu\mathbf{x}(\mathbf{p}-\mathbf{q})}=(2\pi)^3\delta^{(3)}(\mathbf{p}-\mathbf{q})\,,\qquad\phi(t,\mathbf{p})=\int\dt^3x e^{\imagu\mathbf{p}\mathbf{x}}\phi(t,\mathbf{x})
    \end{equation}
\end{subequations}

\begin{subequations}
    \begin{align}
        \overline{\phi}(x^0\equiv t,\mathbf{p}) & =\int\dt^3x e^{\imagu\mathbf{p}\mathbf{x}}\overline{\phi}(x^0\equiv t,\mathbf{x})                                                                                                                                                                                                                                             \\
                                                & =\int\dt^3xe^{\imagu\mathbf{p}\mathbf{x}}\int\dt^4yG_{\text{ret}}(x,y)j(y)                                                                                                                                                                                                                                                    \\
                                                & =\int\dt^3xe^{\imagu\mathbf{p}\mathbf{x}}\int\dt^4y\Theta(x^0-y^0)\big[D(x-y)-D(y-x)\big]j(y)                                                                                                                                                                                                                                 \\
                                                & =\int\dt^3xe^{\imagu\mathbf{p}\mathbf{x}}\int\dt^4y\int\frac{\dt^3q}{(2\pi)^3}\frac{1}{2\omega_{\mathbf{q}}}\Theta(x^0-y^0)\big[e^{-\imagu[w_{\mathbf{q}}(x^0-y^0)-\mathbf{q}(\mathbf{x}-\mathbf{y})]}-e^{\imagu[w_{\mathbf{q}}(x^0-y^0)-\mathbf{q}(\mathbf{x}-\mathbf{y})]}\big]j(y)                                         \\
                                                & =\int\dt^3x\int\dt^4y\int\frac{\dt^3q}{(2\pi)^3}\frac{1}{2\omega_{\mathbf{q}}}\Theta(x^0-y^0)\big[e^{-\imagu[w_{\mathbf{q}}(x^0-y^0)+\mathbf{q}\mathbf{y}]}e^{\imagu(\mathbf{p}+\mathbf{q})\mathbf{x}}-e^{\imagu[w_{\mathbf{q}}(x^0-y^0)+\mathbf{q}\mathbf{y}]}e^{\imagu(\mathbf{p}-\mathbf{q})\mathbf{x}}\big]j(y)           \\
                                                & =\int\dt^4y\int\dt^3q\frac{1}{2\omega_{\mathbf{q}}}\Theta(x^0-y^0)\big[e^{-\imagu[w_{\mathbf{q}}(x^0-y^0)+\mathbf{q}\mathbf{y}]}\delta^{(3)}(\mathbf{p}+\mathbf{q})-e^{\imagu[w_{\mathbf{q}}(x^0-y^0)+\mathbf{q}\mathbf{y}]}\delta^{(3)}(\mathbf{p}-\mathbf{q})\big]j(y)                                                      \\
                                                & =\int\dt^4y\frac{1}{2\omega_{\mathbf{p}}}\Theta(x^0-y^0)\big[e^{-\imagu[w_{\mathbf{p}}(x^0-y^0)-\mathbf{p}\mathbf{y}]}-e^{\imagu[w_{\mathbf{p}}(x^0-y^0)+\mathbf{p}\mathbf{y}]}\big]j(y)                                                                                                                                      \\
                                                & =\int\dt^4y\frac{1}{2\omega_{\mathbf{p}}}\Theta(x^0-y^0)e^{\imagu\mathbf{p}\mathbf{y}}\big[e^{-\imagu\omega_{\mathbf{p}}(x^0-y^0)}-e^{\imagu\omega_{\mathbf{p}}(x^0-y^0)}\big]j(y)                                                                                                                                            \\
                                                & =\int\dt^4y\frac{1}{\imagu\omega_\mathbf{p}}\Theta(x^0-y^0)e^{\imagu\mathbf{p}{\mathbf{y}}}\sin(\omega_{\mathbf{p}}(x^0-y^0))j(y)                                                                                                                                                                                             \\
        \intertext{Specify this for the relevant case $\text{supp}j=\Sigma_{\text{freeze-out}}$ and parametrize the integral over the hypersurface $\Sigma$ via $\int_\Sigma\dt^4y=\int\dt\varphi\dt\eta\dt\alpha r(\alpha)\tau(\alpha)\sqrt{r^{\prime 2}(\alpha)-\tau^{\prime 2}(\alpha)}$}
        \overline{\phi}(x^0\equiv t,\mathbf{p}) & =\int_0^{2\pi}\dt\varphi\int_{-\infty}^\infty\dt\eta\int_0^\pi\dt\alpha r(\alpha)\tau(\alpha)\sqrt{r^{\prime 2}(\alpha)-\tau^{\prime 2}(\alpha)}\frac{1}{\imagu\omega_{\mathbf{p}}}\Theta(x^0-\tau\cosh\eta)\times                                                                                                  \nonumber \\
                                                & \phantom{=}\qquad\times\exp\left(\imagu[\mathbf{p}^\perp\mathbf{x}^\perp+p_z\tau(\alpha)\sinh\eta]\right)\sin(\omega_{\mathbf{p}}(x^0-\tau(\alpha)\cosh\eta))j(\tau(\alpha),r(\alpha))                                                                                                                                        \\
        \intertext{Performing the $\varphi$-integration, with $\varphi$ appearing in the integrand in $\mathbf{x}^\perp=(r\cos\varphi,r\sin\varphi)$, we choose to align $\varphi=0$ with the $\mathbf{p}^\perp=(p_x,p_y)$ direction.Then $\mathbf{p}^\perp\mathbf{x}^\perp=p^\perp r\cos\varphi$. Use the definition of modified Bessel function (\url{https://dlmf.nist.gov/10.32}) $$I_0(z)=\frac{1}{\pi}\int_0^\pi e^{\pm z\cos\theta}\dt\theta$$ the result simplifies to}
        \overline{\phi}(x^0\equiv t,\mathbf{p}) & =\int_{-\infty}^\infty\dt\eta\int_0^\pi\dt\alpha r(\alpha)\tau(\alpha)\sqrt{r^{\prime 2}(\alpha)-\tau^{\prime 2}(\alpha)}\frac{1}{\imagu\omega_{\mathbf{p}}}\Theta(x^0-\tau\cosh\eta)\times                                                                                                  \nonumber                        \\
                                                & \phantom{=}\qquad\times\frac{2}{\pi}I_0(\imagu p^\perp r(\alpha))\exp\left(\imagu p_z\tau(\alpha)\sinh\eta\right)\sin(\omega_{\mathbf{p}}(x^0-\tau(\alpha)\cosh\eta))j(\tau(\alpha),r(\alpha))
    \end{align}
\end{subequations}

\begin{calc}[Metric on Hypersurface]{calc:HypersurfaceMetric}
    Recall the metric $g_{\mu\nu}=\text{diag}(-1,1,\tau^2,r^2)$ in coordinates $(\tau,r,\eta,\varphi)$. Orthonormal tangent vectors to the freeze out hypersurface are $(\hat\partial_\varphi)^\mu=(0,0,0,r^{-1})=r^{-1}(\partial_\varphi)^\mu$, $(\hat\partial_\eta)^\mu=(0,0,\tau^{-1},0)=\tau^{-1}(\partial_\eta)^\mu$ and $(\hat\partial_\alpha)^\mu=\sqrt{r^{\prime 2}(\alpha)-\tau^{\prime 2}(\alpha)}^{-1}(\tau^{\prime}(\alpha),r^{\prime}(\alpha),0,0)=D(\alpha)(\partial_\alpha)^\mu$ with $D(\alpha)=\sqrt{r^{\prime 2}(\alpha)-\tau^{\prime 2}(\alpha)}^{-1}$. The projector on the hypersurface is
    \begin{equation}
        \gamma_{\mu\nu}=(\hat\partial_\varphi)_\mu(\hat\partial_\varphi)_\nu+(\hat\partial_\eta)_\mu(\hat\partial_\eta)_\nu+(\hat\partial_\alpha)_\mu(\hat\partial_\alpha)_\nu=\begin{pmatrix}
            D^2(\alpha)\tau^{\prime2}(\alpha)               & -D^2(\alpha)\tau^\prime(\alpha)r^\prime(\alpha) & 0      & 0   \\
            -D^2(\alpha)\tau^\prime(\alpha)r^\prime(\alpha) & D^2(\alpha)r^{\prime2}(\alpha)                  & 0      & 0   \\
            0                                               & 0                                               & \tau^2 & 0   \\
            0                                               & 0                                               & 0      & r^2
        \end{pmatrix}
    \end{equation}
    The normal of the hypersurface is $n^\mu\equiv(\hat\partial_\alpha^\perp)^\mu=D(\alpha)(r^\prime(\alpha),\tau^\prime(\alpha),0,0)$ and is timelike where $D$ is real. Naturally $\gamma_{\mu\nu}n^\nu=0$. In the basis $(\partial_\alpha,\partial_\eta,\partial_\varphi,n)$ using (in short form)
    \begin{equation}
        (\partial_\alpha)^\nu\gamma_{\mu\nu}(\partial_\alpha)^\mu=\begin{pmatrix}
            \tau^\prime \\r^\prime
        \end{pmatrix}^T\begin{pmatrix}
            -\tau^\prime \\
            r^\prime
        \end{pmatrix}=D^{-2}
    \end{equation}
    the hypersurface metric in coordinates $x^i=(\alpha,\eta,\varphi)$ reads
    \begin{equation}
        \gamma_{ij}=\text{diag}(D^{-2}(\alpha),\tau^2(\alpha),r^2(\alpha))
    \end{equation}
    and the volume element is given by $\dt\Sigma=r(\alpha)\tau(\alpha) D^{-1}(\alpha)\dt\alpha\dt\eta\dt\varphi$. The oriented surface element is \begin{equation}
        \dt\Sigma^\mu=n^\mu\dt\Sigma=r(\alpha)\tau(\alpha)(r^\prime(\alpha),\tau^\prime(\alpha),0,0)\dt\alpha\dt\eta\dt\varphi
    \end{equation}
\end{calc}

\paragraph{Converting Spectra between Coordinate Systems}

Consider the coordinate change in momentum space
\begin{equation}
    \left\{
    \begin{split}
        p_x&=p^\perp\cos\varphi_p\\
        p_y&=p^\perp\sin\varphi_p\\
        p_z&=m^\perp\sinh\eta_p\\
        p_t&=m^\perp\cosh\eta_p
    \end{split}
    \right.\qquad\iff\qquad
    \left\{
    \begin{split}
        p^\perp&=\sqrt{p_x^2+p_y^2}\\
        \varphi_p&=\arctan(p_y/p_y)\\
        m^\perp&=\sqrt{p_t^2-p_z^2}\\
        \eta_p&=\artanh(p_z/p_t)
    \end{split}
    \right.
\end{equation}
with Jacobian
\begin{equation}
    \big\vert\frac{\partial(p^\perp,\varphi_p,m^\perp,\eta_p)}{\partial(p_x,p_y,p_z,p_t)}\big\vert=\frac{1}{m^\perp p^\perp}
\end{equation}
Let $f(p_\mu)$ be some distribution function and $F$ its momentum space integral evaluated on the momentum shell and future directed momenta.

\begin{subequations}
    \begin{align}
        F=\int\frac{\dt^4p_{\text{cart}}}{(2\pi)^4}\delta(p^2-m^2)\Theta(p_t)f(p_\mu) & =\int\frac{\dt p_t}{2\pi}\int\frac{\dt^3p_{\text{cart}}}{(2\pi)^3}\frac{1}{2\omega_{\mathbf{p}}}\big(\delta(p_t-\omega_{\mathbf{p}})+\delta(p_t+\omega_{\mathbf{p}})\big)\Theta(p_t)f(p_\mu) \\
                                                                                      & =\frac{1}{2\pi}\int\frac{\dt^3p_{\text{cart}}}{(2\pi)^3}\frac{1}{2\omega_{\mathbf{p}}}f(p_\mu)\big\vert_{p_t=\omega_{\mathbf{p}}}
    \end{align}
    On the other hand
    \begin{align}
        F=\int\frac{\dt^4p_{\text{cart}}}{(2\pi)^4}\delta(p^2-m^2)\Theta(p_t)f(p_\mu) & =\frac{1}{(2\pi)^4}\int_0^\infty \dt p^\perp\int_0^\infty \dt m^\perp\int_{-\infty}^\infty \dt\eta_p\int_0^{2\pi}\dt\varphi_pm^\perp p^\perp\delta((p^\perp)^2-(m^\perp)^2)f(p_\mu) \\
        \intertext{assume $f(p^\mu)=f(p^\perp,m^\perp,\eta_p)$ and perform the $\varphi$-integraion}
                                                                                      & =\frac{1}{(2\pi)^3}\int_0^\infty\dt m^\perp\int_{-\infty}^\infty\dt\eta_p\frac{m^\perp}{2}f(p_\mu)\big\vert_{m^\perp=p^\perp}
    \end{align}
    leding to the important result
    \begin{equation}
        \frac{1}{2\pi}\int\frac{\dt^3p_{\text{cart}}}{(2\pi)^3}\frac{1}{2\omega_{\mathbf{p}}}f(p_\mu)\big\vert_{p_t=\omega_{\mathbf{p}}}=\frac{1}{(2\pi)^3}\int_0^\infty\dt m^\perp\int_{-\infty}^\infty\dt\eta_p\frac{m^\perp}{2}f(p_\mu)\big\vert_{m^\perp=p^\perp}
    \end{equation}
\end{subequations}

Since the restrictions $p_t=\omega_{\mathbf{p}}$ and $m^\perp=p^\perp$ are equivalent (considering the parametrization that already satisfies $p_t=p^\perp\cosh\eta_p\geq 0$) we find
\begin{equation}
    \omega_{\mathbf{p}}\frac{\dt F}{\dt p_x\dt p_y\dt p_z}=\frac{1}{2\pi m^\perp}\frac{\dt F}{\dt m^\perp\dt\eta_p}
\end{equation}
The result applies to the case
\begin{equation}
    f(p_\mu)\big\vert_{p_t=\omega_{\mathbf{p}}}=2\omega_{\mathbf{p}}\cdot 2\pi\cdot n(\mathbf{p})
\end{equation}
and $F=N$.


\subsection{Fourier Decomposition on Freeze Out Surface???}

Generally a Fourier Ddecomposition to solve the Klein-Gordon equation in terms of $3$-momentum-modes is given by
\begin{equation}
    \phi(x^\mu)=\int\frac{\dt^4p}{(2\pi)^4}\phi(\vec{p})e^{\imagu p_\mu x^\mu}\delta(p^2-m^2)\Theta(p_0)+\text{c.c.}=\frac{1}{2\pi}\int\frac{\dt^3p}{(2\pi)^3}\frac{1}{2\omega_{\vec{p}}}\phi(\vec{p})e^{\imagu(\omega_{\vec{p}}x^0-\vec{p}\vec{x})}+\text{c.c.}
\end{equation}
For simplicity neglect the $+\text{c.c.}$.

Considering a hypersurface $\Sigma$ and using the field data given only on this hypersurface - that is considering the restriction $\phi\vert_{x\in\Sigma}$ - can we reconstruct $\phi(\vec{p})$? The map $\phi(\vec{p})\mapsto\phi(x^\mu\in\Sigma)$ is trivially given by the mode decomposition above. Let $\Sigma=\Sigma_t=\{x^\mu\in\mathbb{R}^{(1,3)}\vert x^0=t=\text{const}\}$ be a slice of constant lab time. Then the map $\phi(x^\mu\in\Sigma_t)\equiv \phi_t(\vec{x})\mapsto\phi(\vec{p})$ is easily found to be
\begin{equation}
    \phi(\vec{p})=(2\pi)(2\omega_{\vec{p}})\int_{\Sigma_t}\dt^3x\phi_t(\vec{x})e^{-\imagu(\omega_{\vec{p}}t-\vec{p}\vec{x})}
\end{equation}
which of course uses the orthogonality relation
\begin{equation}
    \int\dt^nx_{\text{cart}}e^{\imagu (p_\mu-q_\mu)x^\mu}=(2\pi)^n\delta^{(n)}(p-q)
\end{equation}
valid in cartesian coordinates.

We would like to generalize this to arbitrary $\Sigma$. Let $(y^i)_{i=1}^3$ be the coordinates of a parametrization $x^\mu(y^i)$ of $\Sigma$. The naive attempt would be an integral of the form
\begin{equation}
    \phi(\vec{p})\overset{?}{=}(2\pi)(2\omega_{\vec{p}})\int_\Sigma\dt^3y\sqrt{\gamma}\phi(x^\mu(y^i))e^{-\imagu(\omega_{\vec{p}}t(y^i)-\vec{p}\vec{x}(y^i))}
\end{equation}
where $\gamma$ is the induced metric determinant. The relevant example is $\Sigma=\{x^\mu\in\mathbb{R}^{(1,3)}\vert (\tau,r_\perp)=(\tau(\alpha),r_\perp(\alpha))\}$ with $\tau,r_\perp$ defined by the coordinate transformation
\begin{equation}
    \left\{\begin{split}
        t&=\tau\cosh\eta\\
        z&=\tau\sinh\eta\\
        x&=r_\perp\cos\varphi\\
        y&=r_\perp\sin\varphi
    \end{split}\right.
    \qquad\iff\qquad
    \left\{\begin{split}
        \tau&=\sqrt{t^2-z^2}\\
        \eta&=\artanh(z/t)\\
        r_\perp&=\sqrt{x^2+y^2}\\
        \varphi&=\arctan(y/x)
    \end{split}\right.
\end{equation}

Let's first evaluate $p_\mu x^\mu$ in the Bjorken coordinate system. Therefore introduce an analogous coordinate change in momentum space
\begin{equation}
    \left\{\begin{split}
        p_t&=m_\perp\cosh\eta_p\\
        p_z&=m_\perp\sinh\eta_p\\
        p_x&=p_\perp\cos\varphi_p\\
        p_y&=p_\perp\sin\varphi_p
    \end{split}\right.
\end{equation}
to rewrite the scalar product as
\begin{equation}
    p_\mu x^\mu\equiv\tau(p_t\cosh\eta-p_z\sinh\eta)+r_\perp(p_x\cos\varphi+p_y\sin\varphi)=\tau m_\perp\cosh(\eta-\eta_p)-r_\perp p_\perp\cos(\varphi-\varphi_p)
\end{equation}
We used the identities
\begin{equation}
    \cosh(a-b)=\cosh a\cosh b-\sinh a\sinh b\,,\qquad\cos(a-b)=\cos a\cos b+\sin a\sin b
\end{equation}
The integral measure changes according to $\dt^4p_{\text{cart}}=\dt m_\perp\dt p_\perp\dt\eta_p\dt\varphi_p\cdot m_\perp p_\perp$. The momentum shell condition $p^2=m^2$ is equivalently parametrized by $m_\perp^2=p_\perp^2+m^2\eqdef \omega_\perp^2$.

These coordinates are adapted to boost symmetry $\eta\to\eta^\prime$ along the beam direction and rotational symmetry $\varphi\to\varphi^\prime$ around the beam axis. Investigate first the implications on the mode decomposition, by requesting that $(\partial/\partial\eta)\phi(x^\mu)=0=(\partial/\partial\varphi)\phi(x^\mu)$.
\begin{subequations}
    \begin{align}
        \phi(x^\mu) & =\frac{1}{(2\pi)^4}\int_{-\infty}^\infty\dt m_\perp\int_0^\infty\dt p_\perp\int_{-\infty}^\infty\dt\eta_p\int_0^{2\pi}\dt\varphi_p\cdot m_\perp p_\perp\delta(m_\perp^2-\omega_\perp^2)\Theta(m_\perp)\times\nonumber \\
                    & \phantom{=}\qquad\times \phi(p_x(p_\perp,\varphi_p),p_y(p_\perp,\varphi_p),p_z(m_\perp,\eta_p))e^{\imagu(\tau m_\perp\cosh(\eta-\eta_p)-r_\perp p_\perp\cos(\varphi-\varphi_p))}                                      \\
                    & =\frac{1}{(2\pi)^4}\int_{-\infty}^\infty\dt m_\perp\int_0^\infty\dt p_\perp\int_{-\infty}^\infty\dt\eta_p\int_0^{2\pi}\dt\varphi_p\cdot m_\perp p_\perp\delta(m_\perp^2-\omega_\perp^2)\Theta(m_\perp)\times\nonumber \\
                    & \phantom{=}\qquad\times \phi(p_x(p_\perp,\varphi_p+\varphi),p_y(p_\perp,\varphi_p+\varphi),p_z(m_\perp,\eta_p+\eta))e^{\imagu(\tau m_\perp\cosh\eta_p-r_\perp p_\perp\cos\varphi_p)}                                  \\
        \intertext{From this it follows that $\phi(p_x,p_y,p_z)=\phi(p_\perp)=\phi(\sqrt{p_x^2+p_y^2})$ and we can simplify the integral. Let's also evaluate the $\delta$-distribution by using that $\delta(m_\perp^2-\omega_\perp^2)=(1/2\omega_\perp)(\delta(m_\perp-\omega_\perp)+\delta(m_\perp+\omega_\perp))$}
        \phi(x^\mu) & =\frac{1}{(2\pi)^4}\frac{1}{2}\int_0^\infty\dt p_\perp\int_{-\infty}^\infty\dt\eta_p\int_0^{2\pi}\dt\varphi_p\cdot p_\perp\phi(p_\perp)e^{\imagu(\tau \omega_\perp\cosh\eta_p-r_\perp p_\perp\cos\varphi_p)}          \\
                    & =\frac{1}{2}\frac{1}{(2\pi)^4}\int_0^\infty\dt p_\perp p_\perp\phi(p_\perp)\big(2\pi J_0(r_\perp p_\perp)\big)\big(\pi(-Y_0(\tau\omega_\perp)+\imagu J_0(\tau\omega_\perp))\big)
    \end{align}
\end{subequations}
where in the last step the following integral representation of Bessel functions of the first kind $J_0(x)$ and of the second kind $Y_0(x)$ where used \url{https://dlmf.nist.gov/10.9}
\begin{equation}
    J_0(x\in\mathbb{R})=\frac{1}{2\pi}\int_0^{2\pi}\dt t\exp{(\textcolor{red}{\overset{?}{\pm}}\imagu x\cos t)}\,,\quad
    J_0(x>0)=\frac{1}{\pi}\int_{-\infty}^\infty\dt t\sin(x\cosh t)\,,\quad Y_0(x>0)=-\frac{2}{\pi}\dt t\cos(x\cosh t)
\end{equation}

Let us finally come back to the naive idea of extracting a particular Fourier component by convolution of the field in position space with some plane wave. We wish to evaluate integrals of the form
\begin{subequations}
    \begin{align}
        \phi(p_\mu) & \sim\int_\Sigma\dt^3y\sqrt{\gamma}\phi(x^\mu(y^i))\exp\big(\imagu[\tau(\alpha) m_\perp^p\cosh(\eta-\eta_p)-r_\perp(\alpha) p_\perp\cos(\varphi-\varphi_p)]\big)                                                                       \\
                    & \sim\int_\Sigma\dt\alpha\dt\eta\dt\varphi\sqrt{\gamma}\Bigg(\frac{1}{{(2\pi)^4}}\int\dt m_\perp^q\dt q_\perp\dt \eta_q\dt \varphi_q\cdot m_\perp^q q_\perp\delta(m_\perp^2-\omega_\perp^2)\Theta(m_\perp)\phi(q_\perp)\times\nonumber \\
                    & \phantom{=}\quad\times\exp\Big(\imagu\big[\tau(\alpha) (m_\perp^p\cosh(\eta-\eta_p)-m_\perp^q\cosh(\eta-\eta_q))-r_\perp(\alpha) (p_\perp\cos(\varphi-\varphi_p)-q_\perp\cos(\varphi-\varphi_q))\big]\Big)\Bigg)
    \end{align}
\end{subequations}
Eventually $p_\mu$ should be some on-shell momentum. There seems to exist no useful orthonormality condition to extract $\phi(p_\perp)$ from this.

In terms of Bessel function, let $(z_n)_{n\in\mathbb{N}}$ be zeros of $J_\nu$. Then \url{http://physics.ucsc.edu/~peter/116C/bess_orthog.pdf}
\begin{equation}
    \int_0^1\dt tJ_\nu(z_nt)J_\nu(z_mt)=\delta_{nm}\frac{1}{2}\frac{\dt J_\nu(x)}{\dt x}\big\vert_{x=z_n}
\end{equation}
